Example_Finite_Vars.thy
@@ -1,0 +1,111 @@
+theory Example_Finite_Vars
+  imports LValues_Typed "HOL-Word.Word"
+begin
+
+typedef mem = \<open>{f. \<forall>(n::string) (i::nat). f(n,i) \<in> {..i}}\<close>
+  apply (rule exI[of _ \<open>\<lambda>_. 0\<close>]) by auto
+
+definition var_raw0 :: "string \<Rightarrow> nat \<Rightarrow> (mem,nat) lvalue_raw" where
+  "var_raw0 n i = \<lparr> lv_domain = UNIV, lv_range = {..<i},
+    lv_getter = \<lambda>m. Rep_mem m (n,i-1),
+    lv_setter = \<lambda>a m. Abs_mem (fun_upd (Rep_mem m) (n,i-1) a) \<rparr>"
+
+lemma valid_var_raw0:
+  assumes "i \<noteq> 0"
+  shows "LValues.valid_lvalue (var_raw0 n i)"
+  unfolding var_raw0_def apply (rule valid_lvalueI)
+  using Rep_mem Rep_mem_inverse apply auto
+     apply (subst Abs_mem_inverse)
+      apply auto
+   apply (subst Abs_mem_inverse)
+    apply auto
+  by (metis Suc_le_lessD Suc_le_mono Suc_pred assms neq0_conv)
+
+lemma var_raw0_domain[simp]: "lv_domain (var_raw0 n i) = UNIV"
+  by (simp add: var_raw0_def)
+
+lemma var_raw0_range[simp]: "lv_range (var_raw0 n i) = {..<i}"
+  by (simp add: var_raw0_def)
+
+definition some_f where "some_f = (SOME f. bij_betw f {..<card (UNIV::'val::finite set)} (UNIV::'val set))"
+
+lemma bij_some_f: "bij_betw some_f {..<card (UNIV::'val::finite set)} (UNIV::'val set)"
+  unfolding some_f_def
+  apply (rule someI_ex[where P=\<open>\<lambda>f. bij_betw f {..<card (UNIV::'val set)} (UNIV::'val set)\<close>])
+  by (simp add: finite_same_card_bij)
+
+lemma inj_some_f: "inj_on (some_f::_\<Rightarrow>'val::finite) {..<card (UNIV::'val set)}"
+  using bij_betw_imp_inj_on bij_some_f by blast
+
+definition var_raw :: "string \<Rightarrow> (mem,'val::finite) lvalue_raw" where
+  "var_raw n = lvalue_map some_f
+     (var_raw0 n (card (UNIV::'val set)))"
+
+lemma valid_var_raw[simp]:
+  shows "LValues.valid_lvalue (var_raw n)"
+  unfolding var_raw_def
+  apply (rule valid_lvalue_map)
+   apply (rule valid_var_raw0, simp)
+  unfolding var_raw0_def
+  using inj_some_f by simp
+
+lemma range_var_raw[simp]:
+  "lv_range (var_raw n) = UNIV"
+  unfolding var_raw_def apply simp
+  using bij_some_f
+  using bij_betw_imp_surj_on by blast
+
+lemma domain_var_raw[simp]:
+  "lv_domain (var_raw n) = UNIV"
+  unfolding var_raw_def by simp
+
+lift_definition var :: "string \<Rightarrow> (mem,'val::finite) lvalue" is "Some o var_raw"
+  by auto
+
+lemma valid_var[simp]: "valid_lvalue (var n)"
+  apply transfer by auto
+
+lemma compatible_var_raw0:
+  assumes "n \<noteq> m" and "i \<noteq> 0" and "j \<noteq> 0"
+  shows "LValues.compatible_lvalues (var_raw0 n i) (var_raw0 m j)"
+  apply (rule compatible_lvalues.intros)
+     apply (auto simp: assms valid_var_raw0)
+  unfolding var_raw0_def apply (simp add: Rep_mem_inverse)
+  using Rep_mem apply (subst Abs_mem_inverse; auto)
+  using Rep_mem apply (subst Abs_mem_inverse; auto)
+  by (simp add: assms(1) fun_upd_twist)
+
+lemma compatible_var: 
+  "n \<noteq> m \<Longrightarrow> compatible_lvalues (var n) (var m)"
+  apply transfer apply simp
+  unfolding var_raw_def
+  apply (rule lvalue_map_compat1)
+  apply (rule lvalue_map_compat2)
+  apply auto
+    apply (rule compatible_var_raw0)
+  using inj_some_f by auto
+
+definition x::"(mem,bool)lvalue" where "x = var ''x''"
+definition y::"(mem,32 word)lvalue" where "y = var ''y''"
+
+lemma valid_x[simp]: "valid_lvalue x"
+  by (simp add: x_def)
+
+lemma valid_y[simp]: "valid_lvalue y"
+  by (simp add: y_def)
+
+lemma compat_xy[simp]: "compatible_lvalues x y"
+  by (simp add: compatible_var x_def y_def)
+
+lemma compat_yx[simp]: "compatible_lvalues y x"
+  by (simp add: compatible_var x_def y_def)
+
+
+
+lemma test:
+  "getter (lvalue_pair x y) (setter x True (setter y 99 m))
+      = (True, 99)"
+
+  by simp
+
+end
