LValues_Typed.thy
@@ -1,0 +1,85 @@
+theory LValues_Typed
+  imports LValues
+begin
+
+typedef ('mem, 'val) lvalue = \<open>{xopt :: ('mem,'val) lvalue_raw option.
+  case xopt of None \<Rightarrow> True | Some x \<Rightarrow> 
+    valid_lvalue x \<and> lv_range x = UNIV \<and> lv_domain x = UNIV}\<close>
+  by (rule exI[of _ None], simp)
+setup_lifting type_definition_lvalue
+
+lift_definition valid_lvalue :: "('mem,'val) lvalue \<Rightarrow> bool" is "\<lambda>x. x \<noteq> None".
+
+lift_definition compatible_lvalues :: "('mem,'val1) lvalue \<Rightarrow> ('mem,'val2) lvalue \<Rightarrow> bool" is
+  \<open>\<lambda>x y. case (x,y) of (Some x, Some y) \<Rightarrow> LValues.compatible_lvalues x y | _ \<Rightarrow> False\<close>.
+
+lift_definition lvalue_pair :: "('mem,'val1) lvalue \<Rightarrow> ('mem,'val2) lvalue \<Rightarrow> ('mem,'val1\<times>'val2) lvalue" is
+  \<open>\<lambda>x y. case (x,y) of (Some x, Some y) \<Rightarrow> 
+    if LValues.compatible_lvalues x y then Some (LValues.lvalue_pair x y) else None
+    | _ \<Rightarrow> None\<close>
+  apply (rename_tac x y; case_tac x; case_tac y)
+     apply auto
+  apply (simp add: lvalue_pair_def)
+  by (simp add: lvalue_pair_def)
+
+lemma "compatible_lvalues x y \<Longrightarrow> valid_lvalue (lvalue_pair x y)"
+  apply transfer 
+      apply (rename_tac x y; case_tac x; case_tac y)
+  by auto
+
+lemma "compatible_lvalues x y \<Longrightarrow> valid_lvalue x"
+  apply transfer apply (rename_tac x y; case_tac x) by auto
+
+lemma "compatible_lvalues x y \<Longrightarrow> valid_lvalue y"
+  apply transfer apply (rename_tac x y; case_tac x; case_tac y) by auto
+
+lift_definition lvalue_chain :: "('mem,'val1) lvalue \<Rightarrow> ('val1,'val2) lvalue \<Rightarrow> ('mem,'val2) lvalue" is
+  \<open>\<lambda>x y. case (x,y) of (Some x, Some y) \<Rightarrow> Some (LValues.lvalue_chain x y)
+    | _ \<Rightarrow> None\<close>
+  apply (rename_tac x y; case_tac x; case_tac y) by auto
+
+lemma "valid_lvalue x \<Longrightarrow> valid_lvalue y \<Longrightarrow> valid_lvalue (lvalue_chain x y)"
+  apply transfer by auto
+
+lift_definition the_invalid_lvalue :: "('mem,'val) lvalue" is "None"
+  by auto
+
+typedef 'mem memory_rest = "UNIV :: 'mem set set"..
+setup_lifting type_definition_memory_rest
+
+lift_definition split_memory :: "('mem,'val) lvalue \<Rightarrow> 'mem \<Rightarrow> ('val\<times>'mem memory_rest)" is
+  "\<lambda>x m. case x of None \<Rightarrow> (undefined, {m})
+                 | Some x \<Rightarrow> LValues.split_memory x m".
+
+lift_definition setter :: "('mem,'val) lvalue \<Rightarrow> 'val \<Rightarrow> 'mem \<Rightarrow> 'mem" is
+  "\<lambda>x. case x of Some x \<Rightarrow> lv_setter x | None \<Rightarrow> \<lambda>_. id".
+
+lift_definition getter :: "('mem,'val) lvalue \<Rightarrow> 'mem \<Rightarrow> 'val" is
+  "\<lambda>x. case x of Some x \<Rightarrow> lv_getter x | None \<Rightarrow> \<lambda>_. undefined".
+
+lemma getter_pair[simp]:
+  fixes x y
+  assumes "compatible_lvalues x y"
+  shows "getter (lvalue_pair x y) m = (getter x m, getter y m)"
+  using assms apply (transfer fixing: m)
+  apply (rename_tac x y; case_tac x; case_tac y)
+     apply auto
+  by (simp add: LValues.lvalue_pair_def)
+
+lemma getter_setter[simp]:
+  fixes x
+  assumes "valid_lvalue x"
+  shows "getter x (setter x a m) = a"
+  using assms apply (transfer fixing: m)
+  by auto
+
+lemma getter_setter_compat[simp]:
+  fixes x y
+  assumes "compatible_lvalues x y"
+  shows "getter x (setter y a m) = getter x m"
+  using assms apply transfer
+  apply (rename_tac x y a m; case_tac x; case_tac y)
+  by auto
+
+
+end
